Fix examples.

lunarlander/basic.thy
@@ -13,25 +13,24 @@ definition z :: exp where
   "z == RVar ''parz''"
 
 definition Assignment :: proc where 
-  "Assignment == x := ((Con Real 1) [+] x)"
+  "Assignment == x := ((Real 1) [+] x)"
 
 lemma B01:
-  "{x[\<ge>](Con Real 0)} x := ((Con Real 1) [+] x) {x[\<ge>](Con Real 1); elE 0}"
+  "{x[\<ge>](Real 0)} x := ((Real 1) [+] x) {x[\<ge>](Real 1); elE 0}"
   unfolding x_def
   apply (rule AssignRRule, auto, fold x_def)
 proof -
   fix s
-  assume a: "(x[\<ge>]Con Real 0) s"
-  obtain c where evalx: "evalE x s = Real c"
-    using a[unfolded fGreaterEqual_def]
-    apply (cases "evalE x s") by auto
-  show "(x[\<ge>]Con Real 1) (\<lambda>(y, i). if y = ''parx'' \<and> i = R then evalE (Con Real 1 [+] x) s else s (y, i))" 
+  assume a: "(x[\<ge>]Real 0) s"
+  obtain c where evalx: "evalE x s = c"
+    using a[unfolded fGreaterEqual_def] by auto
+  show "(x[\<ge>]Real 1) (\<lambda>y. if y = ''parx'' then evalE (Real 1 [+] x) s else s y)" 
   proof -
-    have eval0: "evalE (Con Real 0) s = Real 0"
+    have eval0: "evalE (Real 0) s = 0"
       by auto
     from a[unfolded fGreaterEqual_def] evalx eval0
     have nonneg_c: "0 \<le> c" by auto
-    have evalx': "s (''parx'', R) = Real c"
+    have evalx': "s ''parx'' = c"
       using evalx unfolding x_def evalE.simps(2) by auto
     show ?thesis
       unfolding fGreaterEqual_def x_def evalE.simps(2) evalE.simps(1)
@@ -40,16 +39,16 @@ proof -
 qed
 
 lemma B02:
-  "{x[\<ge>](Con Real 0)}
-    (x :=((Con Real 1) [+] x ));
-    (x :=((Con Real 1) [+] x ))*&& x[\<ge>](Con Real 1)
-   {x[\<ge>](Con Real 1);elE 0}"
+  "{x[\<ge>](Real 0)}
+    (x :=((Real 1) [+] x ));
+    (x :=((Real 1) [+] x ))*&& x[\<ge>](Real 1)
+   {x[\<ge>](Real 1);elE 0}"
 
-apply (cut_tac p="x[\<ge>](Con Real 0)"
-           and P="(x :=((Con Real 1) [+] x ))" 
-           and m="x[\<ge>](Con Real 1)"
-           and Q="(x :=((Con Real 1) [+] x ))*&& x[\<ge>](Con Real 1)" 
-           and q="x[\<ge>](Con Real 1)"
+apply (cut_tac p="x[\<ge>](Real 0)"
+           and P="(x :=((Real 1) [+] x ))" 
+           and m="x[\<ge>](Real 1)"
+           and Q="(x :=((Real 1) [+] x ))*&& x[\<ge>](Real 1)" 
+           and q="x[\<ge>](Real 1)"
            and H="elE 0"
            and G="elE 0"
             in  SequentialRule_aux,auto)
@@ -57,35 +56,34 @@ apply (cut_tac p="x[\<ge>](Con Real 0)"
    defer
    apply (simp add:chop_def)
   apply (simp add: Valid_def)
-apply (cut_tac I="x[\<ge>](Con Real 1)"
-           and P="x :=((Con Real 1) [+] x )" 
+apply (cut_tac I="x[\<ge>](Real 1)"
+           and P="x :=((Real 1) [+] x )" 
            and H="elE 0" 
             in  RepetitionRule,auto)
 apply (simp add:chop_def) 
 defer
 apply (simp add:dOr_def )
-apply (cut_tac p="x[\<ge>](Con Real 1)" 
-           and q="x[\<ge>](Con Real 1)" 
+apply (cut_tac p="x[\<ge>](Real 1)" 
+           and q="x[\<ge>](Real 1)" 
            and H="elE 0" 
            and x="''parx''" 
-           and f="((Con Real 1) [+] x )" in  AssignRRule,auto)
+           and f="((Real 1) [+] x )" in  AssignRRule,auto)
 defer apply (simp add:x_def)
 
 proof-
   fix s
-  assume a:"(x[\<ge>]Con Real 1) s"
-  obtain c where evalx: "evalE x s = Real c"
-     using a[unfolded fGreaterEqual_def]
-     apply (cases "evalE x s") by auto
-   show "(x[\<ge>]Con Real 1)
-          (\<lambda>(y, i). if y = ''parx'' \<and> i = R then evalE (Con Real 1 [+] x) s else s (y, i))"
+  assume a:"(x[\<ge>]Real 1) s"
+  obtain c where evalx: "evalE x s = c"
+     using a[unfolded fGreaterEqual_def] by auto
+   show "(x[\<ge>]Real 1)
+          (\<lambda>y. if y = ''parx'' then evalE (Real 1 [+] x) s else s y)"
 proof -
-    have eval1: "evalE (Con Real 1) s = Real 1"
+    have eval1: "evalE (Real 1) s = 1"
       by auto
     from a[unfolded fGreaterEqual_def] evalx eval1
     have nonneg_c1: "1 \<le> c" by auto
     have nonneg_c0: "0 \<le> c" using nonneg_c1 by linarith
-    have evalx': "s (''parx'', R) = Real c"
+    have evalx': "s ''parx'' = c"
       using evalx unfolding x_def evalE.simps(2) by auto
     show ?thesis
       unfolding fGreaterEqual_def x_def evalE.simps(2) evalE.simps(1)
@@ -95,15 +93,15 @@ qed
 
 
 lemma B03:
-  "{x[\<ge>](Con Real 0)}
-    (x :=((Con Real 1) [+] x ));
-    (x :=((Con Real 1) [+] x )) [[ (y :=((Con Real 1) [+] y ))
-   {x[\<ge>](Con Real 1);elE 0}"
-apply (cut_tac p="x[\<ge>](Con Real 0)"
-           and P="(x :=((Con Real 1) [+] x ))" 
-           and m="x[\<ge>](Con Real 1)"
-           and Q="(x :=((Con Real 1) [+] x )) [[ (y :=((Con Real 1) [+] y ))" 
-           and q="x[\<ge>](Con Real 1)"
+  "{x[\<ge>](Real 0)}
+    (x :=((Real 1) [+] x ));
+    (x :=((Real 1) [+] x )) [[ (y :=((Real 1) [+] y ))
+   {x[\<ge>](Real 1);elE 0}"
+apply (cut_tac p="x[\<ge>](Real 0)"
+           and P="(x :=((Real 1) [+] x ))" 
+           and m="x[\<ge>](Real 1)"
+           and Q="(x :=((Real 1) [+] x )) [[ (y :=((Real 1) [+] y ))" 
+           and q="x[\<ge>](Real 1)"
            and H="elE 0"
            and G="elE 0"
             in  SequentialRule_aux,auto)
@@ -111,64 +109,62 @@ apply (cut_tac p="x[\<ge>](Con Real 0)"
    defer
    apply (simp add:chop_def)
   apply (simp add: Valid_def)
-  apply (cut_tac P="(x :=((Con Real 1) [+] x )) "
-           and Q="(y :=((Con Real 1) [+] y ))" 
-           and p="x[\<ge>](Con Real 1)" 
-           and m="x[\<ge>](Con Real 1)" 
-           and q="x[\<ge>](Con Real 1)" 
+  apply (cut_tac P="(x :=((Real 1) [+] x )) "
+           and Q="(y :=((Real 1) [+] y ))" 
+           and p="x[\<ge>](Real 1)" 
+           and m="x[\<ge>](Real 1)" 
+           and q="x[\<ge>](Real 1)" 
            and H="elE 0" 
            and G="elE 0"  in JoinRule,auto)
 defer
 defer
 apply (simp add:fOr_def )
 apply (simp add:dOr_def )
-apply (cut_tac p="x[\<ge>](Con Real 1)" 
-           and q="x[\<ge>](Con Real 1)" 
+apply (cut_tac p="x[\<ge>](Real 1)" 
+           and q="x[\<ge>](Real 1)" 
            and H="elE 0" 
            and x="''parx''" 
-           and f="((Con Real 1) [+] x )" in  AssignRRule,auto)
+           and f="((Real 1) [+] x )" in  AssignRRule,auto)
     defer 
     apply (simp add:x_def)
-apply (cut_tac p="x[\<ge>](Con Real 1)" 
-           and q="x[\<ge>](Con Real 1)" 
+apply (cut_tac p="x[\<ge>](Real 1)" 
+           and q="x[\<ge>](Real 1)" 
            and H="elE 0" 
            and x="''pary''" 
-           and f="((Con Real 1) [+] y )" in  AssignRRule,auto)
+           and f="((Real 1) [+] y )" in  AssignRRule,auto)
     defer
     apply (simp add:y_def)
   
 proof-
   fix s
-  assume a:"(x[\<ge>]Con Real 1) s"
-  obtain c where evalx: "evalE x s = Real c"
-     using a[unfolded fGreaterEqual_def]
-     apply (cases "evalE x s") by auto
-   show "(x[\<ge>]Con Real 1)
-          (\<lambda>(y, i). if y = ''parx'' \<and> i = R then evalE (Con Real 1 [+] x) s else s (y, i))"
+  assume a:"(x[\<ge>]Real 1) s"
+  obtain c where evalx: "evalE x s = c"
+     using a[unfolded fGreaterEqual_def] by auto
+   show "(x[\<ge>]Real 1)
+          (\<lambda>y. if y = ''parx'' then evalE (Real 1 [+] x) s else s y)"
 proof -
-    have eval1: "evalE (Con Real 1) s = Real 1"
+    have eval1: "evalE (Real 1) s = 1"
       by auto
     from a[unfolded fGreaterEqual_def] evalx eval1
     have nonneg_c1: "1 \<le> c" by auto
     have nonneg_c0: "0 \<le> c" using nonneg_c1 by linarith
-    have evalx': "s (''parx'', R) = Real c"
+    have evalx': "s ''parx'' = c"
       using evalx unfolding x_def evalE.simps(2) by auto
     show ?thesis
       unfolding fGreaterEqual_def x_def evalE.simps(2) evalE.simps(1)
       by (simp add: evalx' nonneg_c0)
   qed
-  assume a:"(x[\<ge>]Con Real 1) s"
-  obtain c where evalx: "evalE x s = Real c"
-     using a[unfolded fGreaterEqual_def]
-     apply (cases "evalE x s") by auto
-   show "(x[\<ge>]Con Real 1)
-          (\<lambda>(ya, i). if ya = ''pary'' \<and> i = R then evalE (Con Real 1 [+] y) s else s (ya, i)) "
+  assume a:"(x[\<ge>]Real 1) s"
+  obtain c where evalx: "evalE x s = c"
+     using a[unfolded fGreaterEqual_def] by auto
+   show "(x[\<ge>]Real 1)
+          (\<lambda>ya. if ya = ''pary'' then evalE (Real 1 [+] y) s else s ya) "
 proof -
-    have eval1: "evalE (Con Real 1) s = Real 1"
+    have eval1: "evalE (Real 1) s = 1"
       by auto
     from a[unfolded fGreaterEqual_def] evalx eval1
     have nonneg_c1: "1 \<le> c" by auto
-    have evalx': "s (''parx'', R) = Real c"
+    have evalx': "s ''parx'' = c"
       using evalx unfolding x_def evalE.simps(2) by auto
     show ?thesis
       unfolding fGreaterEqual_def x_def y_def evalE.simps(2) evalE.simps(1)
@@ -178,20 +174,20 @@ qed
 
 consts Inv :: fform
 
-definition cons11 :: fform where "cons11 \<equiv> (x [\<ge>] Con Real 1) [\<longrightarrow>] Inv"
-definition cons12 :: fform where "cons12 \<equiv> Inv [\<longrightarrow>] (x [\<ge>] Con Real 1)"
-definition cons13 :: fform where "cons13 \<equiv> exeFlow(<[(''parx'', R)]: [(Con Real 2)] && Inv & fTrue>) Inv [\<longrightarrow>] Inv"
+definition cons11 :: fform where "cons11 \<equiv> (x [\<ge>] Real 1) [\<longrightarrow>] Inv"
+definition cons12 :: fform where "cons12 \<equiv> Inv [\<longrightarrow>] (x [\<ge>] Real 1)"
+definition cons13 :: fform where "cons13 \<equiv> exeFlow(<[''parx'']: [(Real 2)] && Inv & fTrue>) Inv [\<longrightarrow>] Inv"
 
 lemma allcons1: "\<forall>s. (cons11 [&] cons12 [&] cons13) s"
   apply (simp only: cons11_def cons12_def cons13_def x_def)
   sorry
 
 lemma ODE1:
-  "{x [\<ge>] (Con Real 0)}  \<comment> \<open>x >= 0\<close>
-    (x := ((Con Real 1) [+] x));  \<comment> \<open>x := 1 + x\<close>
-    <[(''parx'', R)]: [(Con Real 2)] && Inv & fTrue>  \<comment> \<open>x' = 2 & True\<close>
-   {x[\<ge>](Con Real 1); (elE 0 [[|]] (almost (x[\<ge>](Con Real 1))))}"  \<comment> \<open>x >= 1\<close>
-  apply (rule SequentialRule[where m="x[\<ge>](Con Real 1)" and H="elE 0" and G="elE 0 [[|]] (almost (x[\<ge>](Con Real 1)))"])
+  "{x [\<ge>] (Real 0)}  \<comment> \<open>x >= 0\<close>
+    (x := ((Real 1) [+] x));  \<comment> \<open>x := 1 + x\<close>
+    <[''parx'']: [(Real 2)] && Inv & fTrue>  \<comment> \<open>x' = 2 & True\<close>
+   {x[\<ge>](Real 1); (elE 0 [[|]] (almost (x[\<ge>](Real 1))))}"  \<comment> \<open>x >= 1\<close>
+  apply (rule SequentialRule[where m="x[\<ge>](Real 1)" and H="elE 0" and G="elE 0 [[|]] (almost (x[\<ge>](Real 1)))"])
   apply (rule B01)
   prefer 2 subgoal
     by (simp add:chop_def dOr_def Valid_def)
@@ -199,43 +195,43 @@ lemma ODE1:
   using allcons1 apply (auto simp add: cons11_def cons12_def cons13_def fAnd_def fImp_def dOr_def)
   by (metis (no_types, lifting) almostmono)
 
-definition cons21:: fform where "cons21 \<equiv>  ((x [\<ge>] Con Real 0)[&](y [\<ge>] Con Real 0)[&](z [\<ge>] Con Real 0)) [\<longrightarrow>] Inv "
-definition cons22:: fform where "cons22 \<equiv>  Inv [\<longrightarrow>] (x [\<ge>] Con Real 0) "
-definition cons23:: fform where "cons23 \<equiv>  exeFlow(<[(''parx'', R),(''pary'', R)]: [y,z] && Inv & fTrue>) (Inv)  [\<longrightarrow>]  Inv"
+definition cons21:: fform where "cons21 \<equiv>  ((x [\<ge>] Real 0)[&](y [\<ge>] Real 0)[&](z [\<ge>] Real 0)) [\<longrightarrow>] Inv "
+definition cons22:: fform where "cons22 \<equiv>  Inv [\<longrightarrow>] (x [\<ge>] Real 0) "
+definition cons23:: fform where "cons23 \<equiv>  exeFlow(<[''parx'', ''pary'']: [y,z] && Inv & fTrue>) (Inv)  [\<longrightarrow>]  Inv"
 
 lemma allcons2:"\<forall> s. ( cons21 [&] cons22 [&] cons23 ) s"
   apply (simp only:cons21_def cons22_def cons23_def x_def y_def z_def)
   sorry
 
-lemma ODE2:"{x [\<ge>] Con Real 0 [&] y [\<ge>] Con Real 0 [&] z [\<ge>] Con Real 0}
-           <[(''parx'', R), (''pary'', R)]:[y, z]&&Inv&\<lambda>s. True>
-            {x [\<ge>] Con Real 0; (elE 0 [[|]] (almost (x[\<ge>](Con Real 0))))}"
+lemma ODE2:"{x [\<ge>] Real 0 [&] y [\<ge>] Real 0 [&] z [\<ge>] Real 0}
+           <[''parx'', ''pary'']:[y, z]&&Inv&\<lambda>s. True>
+            {x [\<ge>] Real 0; (elE 0 [[|]] (almost (x[\<ge>](Real 0))))}"
   apply (rule ContinuousRuleGT) 
   using allcons2 apply (auto simp add:cons21_def cons22_def cons23_def x_def y_def z_def fAnd_def fImp_def dOr_def)
   by (smt almostmono)
 
-definition cons31:: fform where "cons31 \<equiv>  (x [\<ge>] Con Real 0) [\<longrightarrow>] Inv "
-definition cons32:: fform where "cons32 \<equiv>  Inv [\<longrightarrow>] (x [\<ge>] Con Real 0) "
-definition cons33:: fform where "cons33 \<equiv>  exeFlow(<[(''parx'', R)]: [(Con Real 5)] && Inv & fTrue>) (Inv)  [\<longrightarrow>]  Inv"
-definition cons34:: fform where "cons34 \<equiv>  exeFlow(<[(''parx'', R)]: [(Con Real 2)] && Inv & fTrue>) (Inv)  [\<longrightarrow>]  Inv"
-definition cons35:: fform where "cons35 \<equiv>  exeFlow(<[(''parx'', R)]: [x] && Inv & fTrue>) (Inv)  [\<longrightarrow>]  Inv"
+definition cons31:: fform where "cons31 \<equiv>  (x [\<ge>] Real 0) [\<longrightarrow>] Inv "
+definition cons32:: fform where "cons32 \<equiv>  Inv [\<longrightarrow>] (x [\<ge>] Real 0) "
+definition cons33:: fform where "cons33 \<equiv>  exeFlow(<[''parx'']: [(Real 5)] && Inv & fTrue>) (Inv)  [\<longrightarrow>]  Inv"
+definition cons34:: fform where "cons34 \<equiv>  exeFlow(<[''parx'']: [(Real 2)] && Inv & fTrue>) (Inv)  [\<longrightarrow>]  Inv"
+definition cons35:: fform where "cons35 \<equiv>  exeFlow(<[''parx'']: [x] && Inv & fTrue>) (Inv)  [\<longrightarrow>]  Inv"
 
 lemma allcons3:"\<forall> s. ( cons31 [&] cons32 [&] cons33 [&] cons34 [&] cons35) s"
   apply (simp only:cons31_def cons32_def cons33_def cons34_def cons35_def
           x_def )
   sorry
 
-lemma ODE3:"{x [\<ge>] Con Real 0 }
-           <[(''parx'', R)]: [(Con Real 5)] && Inv & fTrue>;
-           <[(''parx'', R)]: [(Con Real 2)] && Inv & fTrue>;
-           <[(''parx'', R)]: [x] && Inv & fTrue>
-            {x [\<ge>] Con Real 0; (elE 0 [[|]] (almost (x[\<ge>](Con Real 0))))}"
-  apply (rule SequentialRule[where m="x[\<ge>](Con Real 0)" and H="elE 0 [[|]] (almost (x[\<ge>](Con Real 0)))" and G="elE 0 [[|]] (almost (x[\<ge>](Con Real 0)))"]) 
+lemma ODE3:"{x [\<ge>] Real 0 }
+           <[''parx'']: [(Real 5)] && Inv & fTrue>;
+           <[''parx'']: [(Real 2)] && Inv & fTrue>;
+           <[''parx'']: [x] && Inv & fTrue>
+            {x [\<ge>] Real 0; (elE 0 [[|]] (almost (x[\<ge>](Real 0))))}"
+  apply (rule SequentialRule[where m="x[\<ge>](Real 0)" and H="elE 0 [[|]] (almost (x[\<ge>](Real 0)))" and G="elE 0 [[|]] (almost (x[\<ge>](Real 0)))"]) 
   apply (rule ContinuousRuleGT) 
   using allcons3 apply (simp add:cons31_def cons32_def cons33_def cons34_def cons35_def
           x_def fAnd_def fImp_def dOr_def )
     apply (smt almostmono)
-   apply (rule SequentialRule[where m="x[\<ge>](Con Real 0)" and H="elE 0 [[|]] (almost (x[\<ge>](Con Real 0)))" and G="elE 0 [[|]] (almost (x[\<ge>](Con Real 0)))"]) 
+   apply (rule SequentialRule[where m="x[\<ge>](Real 0)" and H="elE 0 [[|]] (almost (x[\<ge>](Real 0)))" and G="elE 0 [[|]] (almost (x[\<ge>](Real 0)))"]) 
    apply (rule ContinuousRuleGT) 
   using allcons3 apply (simp add:cons31_def cons32_def cons33_def cons34_def cons35_def
           x_def fAnd_def fImp_def dOr_def )
@@ -249,50 +245,50 @@ lemma ODE3:"{x [\<ge>] Con Real 0 }
   done
 
 definition exp41:: exp where
-  "exp41 \<equiv> ((Con Real 0 [-] x [-] ((Con Real 1117 [*] y) [div] Con Real 500)) [+]
-   ((Con Real 439 [*] y [**] 3) [div] Con Real 200 ))[-]((Con Real 333 [*] y [**] 5) [div] Con Real 500) "
+  "exp41 \<equiv> ((Real 0 [-] x [-] ((Real 1117 [*] y) [div] Real 500)) [+]
+   ((Real 439 [*] y [**] 3) [div] Real 200 ))[-]((Real 333 [*] y [**] 5) [div] Real 500) "
 
 definition exp42:: exp where
-  "exp42 \<equiv> ((x [+]((Con Real 617 [*] y) [div] Con Real 500)) [-]
-   ((Con Real 439 [*] y [**] 3) [div] Con Real 200 ))[+]((Con Real 333 [*] y [**] 5) [div] Con Real 500)"
+  "exp42 \<equiv> ((x [+]((Real 617 [*] y) [div] Real 500)) [-]
+   ((Real 439 [*] y [**] 3) [div] Real 200 ))[+]((Real 333 [*] y [**] 5) [div] Real 500)"
 
 definition cons41:: fform where
-  "cons41 \<equiv>  (x[**]2 [\<le>] Con Real (1/2) [&] y[**]2 [\<le>] Con Real (1/3)) [\<longrightarrow>] Inv "
+  "cons41 \<equiv>  (x[**]2 [\<le>] Real (1/2) [&] y[**]2 [\<le>] Real (1/3)) [\<longrightarrow>] Inv "
 
 definition cons42:: fform where
-  "cons42 \<equiv>  Inv [\<longrightarrow>] (x [-] Con Real 4 [*] y [<] Con Real 8) "
+  "cons42 \<equiv>  Inv [\<longrightarrow>] (x [-] Real 4 [*] y [<] Real 8) "
 
 definition cons43:: fform where
-  "cons43 \<equiv>  exeFlow(<[(''parx'', R),(''pary'', R)]: [(exp41),(exp42)] && Inv & fTrue>) (Inv)  [\<longrightarrow>]  Inv"
+  "cons43 \<equiv>  exeFlow(<[''parx'', ''pary'']: [(exp41),(exp42)] && Inv & fTrue>) (Inv)  [\<longrightarrow>]  Inv"
 
 lemma allcons4:"\<forall> s. ( cons41 [&] cons42 [&] cons43 ) s"
   apply (simp only:cons41_def cons42_def cons43_def exp41_def exp42_def
           x_def y_def)
   by (inv_check_oracle "parx^2 + parx*pary + pary^2 - 111/59 <= 0")
 
-lemma ODE4:"{x[**]2 [\<le>] Con Real (1/2) [&] y[**]2 [\<le>] Con Real (1/3)}
-           <[(''parx'', R),(''pary'', R)]: [(exp41),(exp42)] && Inv & fTrue>
-            {x [-] Con Real 4 [*] y [<] Con Real 8;elE 0 [[|]] (almost (x [-] Con Real 4 [*] y [<] Con Real 8))}"
+lemma ODE4:"{x[**]2 [\<le>] Real (1/2) [&] y[**]2 [\<le>] Real (1/3)}
+           <[''parx'', ''pary'']: [(exp41),(exp42)] && Inv & fTrue>
+            {x [-] Real 4 [*] y [<] Real 8;elE 0 [[|]] (almost (x [-] Real 4 [*] y [<] Real 8))}"
   apply (rule ContinuousRuleGT) 
   using allcons4 apply (simp add: cons41_def cons42_def cons43_def x_def y_def fAnd_def fImp_def dOr_def )
   by (smt almostmono)
 
 definition cons51:: fform where
-  "cons51 \<equiv>  (x[**]2 [\<le>] Con Real (1/2) [&] (y [+] Con Real 2)[**]2 [\<le>] Con Real (1/3)) [\<longrightarrow>] Inv"
+  "cons51 \<equiv>  (x[**]2 [\<le>] Real (1/2) [&] (y [+] Real 2)[**]2 [\<le>] Real (1/3)) [\<longrightarrow>] Inv"
 
 definition cons52:: fform where
-  "cons52 \<equiv>  Inv [\<longrightarrow>] ((x [-] Con Real 1) [**]2 [+] (y [-] Con Real (3/2)) [**]2 [>] Con Real (1/4)) "
+  "cons52 \<equiv>  Inv [\<longrightarrow>] ((x [-] Real 1) [**]2 [+] (y [-] Real (3/2)) [**]2 [>] Real (1/4)) "
 
 definition cons53:: fform where
-  "cons53 \<equiv>  exeFlow(<[(''parx'', R),(''pary'', R)]: [((y[-]x)[-]x[**]3),((y[**]2[-]x)[-]y)] && Inv & fTrue>) (Inv)  [\<longrightarrow>]  Inv"
+  "cons53 \<equiv>  exeFlow(<[''parx'', ''pary'']: [((y[-]x)[-]x[**]3),((y[**]2[-]x)[-]y)] && Inv & fTrue>) (Inv)  [\<longrightarrow>]  Inv"
 
 lemma allcons5:"\<forall> s. ( cons51 [&] cons52 [&] cons53 ) s"
   apply (simp only: cons51_def cons52_def cons53_def x_def y_def)
   by (inv_check_oracle "2*(parx^2) + (pary+3/2)^2 - 4 <= 0")
 
-lemma ODE5:"{x[**]2 [\<le>] Con Real (1/2) [&] (y [+] Con Real 2) [**]2 [\<le>] Con Real (1/3)}
-           <[(''parx'', R),(''pary'', R)]: [((y[-]x)[-]x[**]3),((y[**]2[-]x)[-]y)] && Inv & fTrue>
-            {(x [-] Con Real 1) [**]2 [+] (y [-] Con Real (3/2)) [**]2 [>] Con Real (1/4);elE 0 [[|]] (almost ((x [-] Con Real 1) [**]2 [+] (y [-] Con Real (3/2)) [**]2 [>] Con Real (1/4)))}"
+lemma ODE5:"{x[**]2 [\<le>] Real (1/2) [&] (y [+] Real 2) [**]2 [\<le>] Real (1/3)}
+           <[''parx'', ''pary'']: [((y[-]x)[-]x[**]3),((y[**]2[-]x)[-]y)] && Inv & fTrue>
+            {(x [-] Real 1) [**]2 [+] (y [-] Real (3/2)) [**]2 [>] Real (1/4);elE 0 [[|]] (almost ((x [-] Real 1) [**]2 [+] (y [-] Real (3/2)) [**]2 [>] Real (1/4)))}"
 apply (rule ContinuousRuleGT) 
   using allcons5 apply (simp add:cons51_def cons52_def cons53_def 
           x_def y_def  fAnd_def fImp_def dOr_def )
@@ -300,13 +296,13 @@ apply (rule ContinuousRuleGT)
 
 
 definition cons61:: fform where
-  "cons61 \<equiv>  (x[**]2 [=] Con Real 1 [&] y[**]2 [=] Con Real 1 [&] z[**]2 [=] Con Real 1 ) [\<longrightarrow>] Inv "
+  "cons61 \<equiv>  (x[**]2 [=] Real 1 [&] y[**]2 [=] Real 1 [&] z[**]2 [=] Real 1 ) [\<longrightarrow>] Inv "
 
 definition cons62:: fform where
-  "cons62 \<equiv>  Inv [\<longrightarrow>] (([\<not>]x[=]Con Real 0) [&] ([\<not>]y[=]Con Real 0) [&] ([\<not>]z[=]Con Real 0)) "
+  "cons62 \<equiv>  Inv [\<longrightarrow>] (([\<not>]x[=]Real 0) [&] ([\<not>]y[=]Real 0) [&] ([\<not>]z[=]Real 0)) "
 
 definition cons63:: fform where
-  "cons63 \<equiv>  exeFlow(<[(''parx'', R),(''pary'', R),(''parz'',R)]: [(x[*]y[-]x[*]z),(y[*]z[-]y[*]x),(z[*]x[-]z[*]y)] && Inv & fTrue>) (Inv)  [\<longrightarrow>]  Inv"
+  "cons63 \<equiv>  exeFlow(<[''parx'', ''pary'', ''parz'']: [(x[*]y[-]x[*]z),(y[*]z[-]y[*]x),(z[*]x[-]z[*]y)] && Inv & fTrue>) (Inv)  [\<longrightarrow>]  Inv"
 
 lemma allcons6:"\<forall> s. ( cons61 [&] cons62 [&] cons63 ) s"
   apply (simp only:cons61_def cons62_def cons63_def 
@@ -314,9 +310,9 @@ lemma allcons6:"\<forall> s. ( cons61 [&] cons62 [&] cons63 ) s"
   sorry
 
 
-lemma ODE6:"{x[**]2 [=] Con Real 1 [&] y[**]2 [=] Con Real 1 [&] z[**]2 [=] Con Real 1}
-           <[(''parx'', R),(''pary'', R),(''parz'',R)]: [(x[*]y[-]x[*]z),(y[*]z[-]y[*]x),(z[*]x[-]z[*]y)] && Inv & fTrue>
-            {([\<not>]x[=]Con Real 0) [&] ([\<not>]y[=]Con Real 0) [&] ([\<not>]z[=]Con Real 0);elE 0 [[|]] (almost (([\<not>]x[=]Con Real 0) [&] ([\<not>]y[=]Con Real 0) [&] ([\<not>]z[=]Con Real 0)))}"
+lemma ODE6:"{x[**]2 [=] Real 1 [&] y[**]2 [=] Real 1 [&] z[**]2 [=] Real 1}
+           <[''parx'', ''pary'', ''parz'']: [(x[*]y[-]x[*]z),(y[*]z[-]y[*]x),(z[*]x[-]z[*]y)] && Inv & fTrue>
+            {([\<not>]x[=]Real 0) [&] ([\<not>]y[=]Real 0) [&] ([\<not>]z[=]Real 0);elE 0 [[|]] (almost (([\<not>]x[=]Real 0) [&] ([\<not>]y[=]Real 0) [&] ([\<not>]z[=]Real 0)))}"
 apply (rule ContinuousRuleGT) 
   using allcons6 apply (simp add:cons61_def cons62_def cons63_def 
           x_def y_def  fAnd_def fImp_def dOr_def )
@@ -328,13 +324,13 @@ definition Inv2 :: fform where
 "Inv2 == Inv"
 
 definition cons71:: fform where
-  "cons71 \<equiv>  (x[>]Con Real 0 ) [\<longrightarrow>] Inv"
+  "cons71 \<equiv>  (x[>]Real 0 ) [\<longrightarrow>] Inv"
 
 definition cons72:: fform where
-  "cons72 \<equiv>  Inv  [\<longrightarrow>] (x[>]Con Real 0) "
+  "cons72 \<equiv>  Inv  [\<longrightarrow>] (x[>]Real 0) "
 
 definition cons73:: fform where
-  "cons73 \<equiv>  exeFlow(<[(''parx'', R)]: [(Con Real 0)] && Inv & fTrue>) (Inv)  [\<longrightarrow>]  Inv"
+  "cons73 \<equiv>  exeFlow(<[''parx'']: [(Real 0)] && Inv & fTrue>) (Inv)  [\<longrightarrow>]  Inv"
 
 lemma allcons7:"\<forall> s. ( cons71 [&] cons72 [&] cons73 ) s"
   apply (simp only: cons71_def cons72_def cons73_def x_def y_def)
