lunarlander/coaster.thy
@@ -68,43 +68,43 @@ definition a :: exp where
 consts Inv :: fform
 
 definition pre1 :: fform where
-"pre1 == (Con Real g[\<ge>] Con Real 0)
-      [&](v[>]Con Real 0)
-      [&](v[**]2 [+] Con Real (2*g) [*] y [=]Con Real (2*g*yG))
-      [&] (x[\<le>]Con Real x1 [&] x[\<ge>]Con Real x0 [&] y[\<le>] Con Real y1 [&] y[\<ge>] Con Real y0)
-      [&]((Con Real dy0[\<le>]Con Real 0 [&] x[\<le>]Con Real x1 [&] x[\<ge>]Con Real x0 [&] y[\<le>] Con Real y1 [&] y[\<ge>] Con Real y0) 
-        [\<longrightarrow>](v[**]2[\<ge>]Con Real vLo [&] v[**]2[\<le>]Con Real vHi [&] Con Real (dyLo*g)[\<le>] Con Real (-dy0*g)[&]Con Real (-dy0*g)[\<le>]Con Real (dyHi*g)[&] Con Real dx0[*]y [=] Con Real dy0[*]x [+] Con Real (dx0*c)))
-      [&](Con Real dy0[\<le>]Con Real 0)
-      [&]((x[\<le>]Con Real x1 [&] x[\<ge>]Con Real x0 [&] y[\<le>] Con Real y1 [&] y[\<ge>] Con Real y0)[\<longrightarrow>](Con Real dx0[*]v[**]2[>]Con Real (2*dy0*g)[*](Con Real x1[-]x)))
-      [&](Con Real x1[>]Con Real x0)
-      [&](Con Real (dx0^2+dy0^2)[=]Con Real 1)
-      [&](Con Real dx0[>]Con Real 0)"
+"pre1 == (Real g[\<ge>] Real 0)
+      [&](v[>]Real 0)
+      [&](v[**]2 [+] Real (2*g) [*] y [=]Real (2*g*yG))
+      [&] (x[\<le>]Real x1 [&] x[\<ge>]Real x0 [&] y[\<le>] Real y1 [&] y[\<ge>] Real y0)
+      [&]((Real dy0[\<le>]Real 0 [&] x[\<le>]Real x1 [&] x[\<ge>]Real x0 [&] y[\<le>] Real y1 [&] y[\<ge>] Real y0) 
+        [\<longrightarrow>](v[**]2[\<ge>]Real vLo [&] v[**]2[\<le>]Real vHi [&] Real (dyLo*g)[\<le>] Real (-dy0*g)[&]Real (-dy0*g)[\<le>]Real (dyHi*g)[&] Real dx0[*]y [=] Real dy0[*]x [+] Real (dx0*c)))
+      [&](Real dy0[\<le>]Real 0)
+      [&]((x[\<le>]Real x1 [&] x[\<ge>]Real x0 [&] y[\<le>] Real y1 [&] y[\<ge>] Real y0)[\<longrightarrow>](Real dx0[*]v[**]2[>]Real (2*dy0*g)[*](Real x1[-]x)))
+      [&](Real x1[>]Real x0)
+      [&](Real (dx0^2+dy0^2)[=]Real 1)
+      [&](Real dx0[>]Real 0)"
 
 definition post1 :: fform where
-"post1 == (v[>]Con Real 0)
-      [&](v[**]2 [+] Con Real (2*g) [*] y [=]Con Real (2*g*yG))
-      [&](x[\<le>]Con Real x1 [&] x[\<ge>]Con Real x0)
-      [&](Con Real dx0[*]y [=] Con Real dy0[*]x [+] Con Real (dx0*c))"
+"post1 == (v[>]Real 0)
+      [&](v[**]2 [+] Real (2*g) [*] y [=]Real (2*g*yG))
+      [&](x[\<le>]Real x1 [&] x[\<ge>]Real x0)
+      [&](Real dx0[*]y [=] Real dy0[*]x [+] Real (dx0*c))"
 
 definition Inv1 :: fform where
-"Inv1 == (v[>]Con Real 0)
-      [&](v[**]2 [+] Con Real (2*g) [*] y [=]Con Real (2*g*yG))
-      [&]Con Real dx0[*]y [=] Con Real dy0[*]x [+] Con Real (dx0*c)"
+"Inv1 == (v[>]Real 0)
+      [&](v[**]2 [+] Real (2*g) [*] y [=]Real (2*g*yG))
+      [&]Real dx0[*]y [=] Real dy0[*]x [+] Real (dx0*c)"
 
 
 
 definition cons11 :: fform where
 "cons11 == pre1 [\<longrightarrow>] Inv"
 definition cons12 :: fform where
-"cons12 == Inv[&]close(x[\<le>]Con Real x1 [&] x[\<ge>]Con Real x0 [&] y[\<le>] Con Real y1 [&] y[\<ge>] Con Real y0)[\<longrightarrow>]post1"
+"cons12 == Inv[&]close(x[\<le>]Real x1 [&] x[\<ge>]Real x0 [&] y[\<le>] Real y1 [&] y[\<ge>] Real y0)[\<longrightarrow>]post1"
 definition cons13 :: fform where
-"cons13 ==  (exeFlow(<[(''parx'', R),(''pary'',R),(''parv'',R)]: [(v[*]Con Real dx0),(v[*]Con Real dy0),(Con Real (-dy0*g))] && Inv & (x[\<le>]Con Real x1 [&] x[\<ge>]Con Real x0 [&] y[\<le>] Con Real y1 [&] y[\<ge>] Con Real y0)>) (Inv)  [\<longrightarrow>]  Inv )"
+"cons13 ==  (exeFlow(<[''parx'', ''pary'', ''parv'']: [(v[*]Real dx0),(v[*]Real dy0),(Real (-dy0*g))] && Inv & (x[\<le>]Real x1 [&] x[\<ge>]Real x0 [&] y[\<le>] Real y1 [&] y[\<ge>] Real y0)>) (Inv)  [\<longrightarrow>]  Inv )"
 lemma allcons1: "\<forall>s. (cons11[&]cons12 [&] cons13 ) s"
   apply (simp add: cons11_def cons12_def cons13_def  x_def y_def v_def pre1_def post1_def)
   by (inv_check_oracle "g > 0 & dy0 <= 0 & parv > 0 & parv^2 + 2*g*pary - 2*g*yG = 0 & dx0*pary - dy0*parx - dx0*c = 0 ")
 
 lemma linedown:"{pre1}
-             <[(''parx'', R),(''pary'',R),(''parv'',R)]: [(v[*]Con Real dx0),(v[*]Con Real dy0),(Con Real (-dy0*g))] && Inv & (x[\<le>]Con Real x1 [&] x[\<ge>]Con Real x0 [&] y[\<le>] Con Real y1 [&] y[\<ge>] Con Real y0)>
+             <[''parx'', ''pary'', ''parv'']: [(v[*]Real dx0),(v[*]Real dy0),(Real (-dy0*g))] && Inv & (x[\<le>]Real x1 [&] x[\<ge>]Real x0 [&] y[\<le>] Real y1 [&] y[\<ge>] Real y0)>
               {post1;(elE 0 [[|]] (almost post1))}"
   apply (rule ContinuousRuleGT )
   apply auto
@@ -130,153 +130,150 @@ apply (cut_tac allcons1)
 
 
 definition pre2 :: fform where
-"pre2 == (Con Real g[\<ge>] Con Real 0)
-      [&](v[>]Con Real 0)
-      [&](v[**]2 [+] Con Real (2*g) [*] y [=]Con Real (2*g*yG))
-      [&] (x[\<le>]Con Real x1 [&] x[\<ge>]Con Real x0 [&] y[\<le>] Con Real y1 [&] y[\<ge>] Con Real y0)
-      [&]((Con Real dy0[\<ge>]Con Real 0 [&] x[\<le>]Con Real x1 [&] x[\<ge>]Con Real x0 [&] y[\<le>] Con Real y1 [&] y[\<ge>] Con Real y0) 
-        [\<longrightarrow>](v[**]2[\<ge>]Con Real vLo [&] v[**]2[\<le>]Con Real vHi [&] Con Real (dyLo*g)[\<le>] Con Real (-dy0*g)[&]Con Real (-dy0*g)[\<le>]Con Real (dyHi*g)[&] Con Real dx0[*]y [=] Con Real dy0[*]x [+] Con Real (dx0*c)))
-      [&](Con Real dy0[\<ge>]Con Real 0)
-      [&]((x[\<le>]Con Real x1 [&] x[\<ge>]Con Real x0 [&] y[\<le>] Con Real y1 [&] y[\<ge>] Con Real y0)[\<longrightarrow>](Con Real dx0[*]v[**]2[>]Con Real (2*dy0*g)[*](Con Real x1[-]x)))
-      [&](Con Real x1[>]Con Real x0)
-      [&](Con Real (dx0^2+dy0^2)[=]Con Real 1)
-      [&](Con Real dx0[>]Con Real 0)
+"pre2 == (Real g[\<ge>] Real 0)
+      [&](v[>]Real 0)
+      [&](v[**]2 [+] Real (2*g) [*] y [=]Real (2*g*yG))
+      [&] (x[\<le>]Real x1 [&] x[\<ge>]Real x0 [&] y[\<le>] Real y1 [&] y[\<ge>] Real y0)
+      [&]((Real dy0[\<ge>]Real 0 [&] x[\<le>]Real x1 [&] x[\<ge>]Real x0 [&] y[\<le>] Real y1 [&] y[\<ge>] Real y0) 
+        [\<longrightarrow>](v[**]2[\<ge>]Real vLo [&] v[**]2[\<le>]Real vHi [&] Real (dyLo*g)[\<le>] Real (-dy0*g)[&]Real (-dy0*g)[\<le>]Real (dyHi*g)[&] Real dx0[*]y [=] Real dy0[*]x [+] Real (dx0*c)))
+      [&](Real dy0[\<ge>]Real 0)
+      [&]((x[\<le>]Real x1 [&] x[\<ge>]Real x0 [&] y[\<le>] Real y1 [&] y[\<ge>] Real y0)[\<longrightarrow>](Real dx0[*]v[**]2[>]Real (2*dy0*g)[*](Real x1[-]x)))
+      [&](Real x1[>]Real x0)
+      [&](Real (dx0^2+dy0^2)[=]Real 1)
+      [&](Real dx0[>]Real 0)
           "
 
 definition post2 :: fform where
-"post2 == (v[>]Con Real 0)
-      [&](v[**]2 [+] Con Real (2*g) [*] y [=]Con Real (2*g*yG))
-      [&]x[\<le>]Con Real x1 [&] x[\<ge>]Con Real x0
-      [&]Con Real dx0[*]y [=] Con Real dy0[*]x [+] Con Real (dx0*c)
+"post2 == (v[>]Real 0)
+      [&](v[**]2 [+] Real (2*g) [*] y [=]Real (2*g*yG))
+      [&]x[\<le>]Real x1 [&] x[\<ge>]Real x0
+      [&]Real dx0[*]y [=] Real dy0[*]x [+] Real (dx0*c)
       "
 definition cons21 :: fform where
-"cons21 == pre2[&](v[*](a[**]2)[=]Con Real 1) [\<longrightarrow>] Inv"
+"cons21 == pre2[&](v[*](a[**]2)[=]Real 1) [\<longrightarrow>] Inv"
 definition cons22 :: fform where
-"cons22 == Inv[&]close(x[\<le>]Con Real x1 [&] x[\<ge>]Con Real x0 [&] y[\<le>] Con Real y1 [&] y[\<ge>] Con Real y0)[\<longrightarrow>]post2[&](v[*](a[**]2)[=]Con Real 1) "
+"cons22 == Inv[&]close(x[\<le>]Real x1 [&] x[\<ge>]Real x0 [&] y[\<le>] Real y1 [&] y[\<ge>] Real y0)[\<longrightarrow>]post2[&](v[*](a[**]2)[=]Real 1) "
 definition cons23 :: fform where
-"cons23 ==  (exeFlow(<[(''parx'', R),(''pary'',R),(''parv'',R),(''para'',R)]: [(v[*]Con Real dx0),(v[*]Con Real dy0),(Con Real (-dy0*g)),(Con Real (dy0 * g/2) [*] a [div] v)] && Inv & (x[\<le>]Con Real x1 [&] x[\<ge>]Con Real x0 [&] y[\<le>] Con Real y1 [&] y[\<ge>] Con Real y0)>) (Inv)  [\<longrightarrow>]  Inv )"
+"cons23 ==  (exeFlow(<[''parx'', ''pary'', ''parv'', ''para'']: [(v[*]Real dx0),(v[*]Real dy0),(Real (-dy0*g)),(Real (dy0 * g/2) [*] a [div] v)] && Inv & (x[\<le>]Real x1 [&] x[\<ge>]Real x0 [&] y[\<le>] Real y1 [&] y[\<ge>] Real y0)>) (Inv)  [\<longrightarrow>]  Inv )"
 
 lemma allcons2: "\<forall>s. (cons21[&]cons22[&] cons23 ) s"
   apply (simp add: cons21_def cons22_def cons23_def  x_def y_def v_def a_def pre2_def post2_def)
 by (inv_check_oracle "parv*para^2 - 1 = 0 & v^2 + 2*g*y - 2*g*yG = 0 & v > 0 & dx0*y - dy0*x -dx0*c = 0")
-lemma lineuple:"{pre2[&](v[*](a[**]2)[=]Con Real 1)}
-              <[(''parx'', R),(''pary'',R),(''parv'',R),(''para'',R)]: [(v[*]Con Real dx0),(v[*]Con Real dy0),(Con Real (-dy0*g)),(Con Real (dy0 * g/2) [*] a [div] v)] && Inv & (x[\<le>]Con Real x1 [&] x[\<ge>]Con Real x0 [&] y[\<le>] Con Real y1 [&] y[\<ge>] Con Real y0)>
-              {post2[&](v[*](a[**]2)[=]Con Real 1);(elE 0)[[|]]almost (post2[&](v[*](a[**]2)[=]Con Real 1))}"
+lemma lineuple:"{pre2[&](v[*](a[**]2)[=]Real 1)}
+              <[''parx'', ''pary'', ''parv'', ''para'']: [(v[*]Real dx0),(v[*]Real dy0),(Real (-dy0*g)),(Real (dy0 * g/2) [*] a [div] v)] && Inv & (x[\<le>]Real x1 [&] x[\<ge>]Real x0 [&] y[\<le>] Real y1 [&] y[\<ge>] Real y0)>
+              {post2[&](v[*](a[**]2)[=]Real 1);(elE 0)[[|]]almost (post2[&](v[*](a[**]2)[=]Real 1))}"
   sorry
 lemma lineup:"{pre2}
-              <[(''parx'', R),(''pary'',R),(''parv'',R)]: [(v[*]Con Real dx0),(v[*]Con Real dy0),(Con Real (-dy0*g))] && Inv & (x[\<le>]Con Real x1 [&] x[\<ge>]Con Real x0 [&] y[\<le>] Con Real y1 [&] y[\<ge>] Con Real y0)>
+              <[''parx'', ''pary'', ''parv'']: [(v[*]Real dx0),(v[*]Real dy0),(Real (-dy0*g))] && Inv & (x[\<le>]Real x1 [&] x[\<ge>]Real x0 [&] y[\<le>] Real y1 [&] y[\<ge>] Real y0)>
               {post2;(elE 0)[[|]]almost post2}"
-  apply (rule GhostRule[where w="(''para'',R)"
-                          and F="(Con Real (dy0 * g/2) [*] a [div] v)"
-                          and pre="pre2[&](v[*](a[**]2)[=]Con Real 1)"
-                          and post="post2[&](v[*](a[**]2)[=]Con Real 1)"
-                          and HF="(elE 0)[[|]]almost (post2[&](v[*](a[**]2)[=]Con Real 1))"])
+  apply (rule GhostRule[where w="''para''"
+                          and F="(Real (dy0 * g/2) [*] a [div] v)"
+                          and pre="pre2[&](v[*](a[**]2)[=]Real 1)"
+                          and post="post2[&](v[*](a[**]2)[=]Real 1)"
+                          and HF="(elE 0)[[|]]almost (post2[&](v[*](a[**]2)[=]Real 1))"])
          apply auto
   apply(simp add:pre2_def fAnd_def fGreaterEqual_def fLessEqual_def fOr_def fImp_def fEqual_def fLess_def fGreater_def fNot_def)
-lemma lineup:"{pre2}
-             <[(''x'', R),(''y'',R),(''v'',R)]: [(v[*]Con Real dx0),(v[*]Con Real dy0),(Con Real (-dy0*g))] && Inv & (x[\<le>]Con Real x1 [&] x[\<ge>]Con Real x0 [&] y[\<le>] Con Real y1 [&] y[\<ge>] Con Real y0)>
-              {post2;(elE 0 [[|]] (almost post2))}"
   sorry
 
 
 
 definition pre3 :: fform where
-"pre3 == (Con Real g[\<ge>] Con Real 0)
-      [&](v[>]Con Real 0)
-      [&](v[**]2 [+] Con Real (2*g) [*] y [=]Con Real (2*g*yG))
-      [&]((Con Real dy0[\<le>]Con Real 0 [&] x[\<le>]Con Real x1 [&] x[\<ge>]Con Real x0 [&] y[\<le>] Con Real y0 [&] y[\<ge>] Con Real y1)
-       [\<longrightarrow>](((x[-]Con Real cx)[**]2[+](y[-]Con Real cy)[**]2) [=] Con Real r [**]2 [&] x[\<ge>] Con Real cx[&] y[\<ge>] Con Real cy[&]v[**]2[\<ge>]Con Real vLo [&] v[**]2[\<le>]Con Real vHi [&] Con Real centLo[\<le>] Con Real cent[&]Con Real cent [\<le>]Con Real centHi [&] Con Real tanLo[\<le>]Con Real tan[&] Con Real tan[\<le>] Con Real tanHi))
-      [&](Con Real dy0[\<le>]Con Real 0)
-      [&](dx[=](y[-]Con Real cy)[div]Con Real r)
-      [&](dy[=](Con Real cx[-]x)[div]Con Real r)
-      [&](Con Real x1[>]Con Real x0)
-      [&](Con Real y1[<]Con Real y0)
-      [&](Con Real cy[\<le>]Con Real y1)
-      [&](Con Real cx[\<le>]Con Real x0)
-      [&](Con Real r[>]Con Real 0) "
+"pre3 == (Real g[\<ge>] Real 0)
+      [&](v[>]Real 0)
+      [&](v[**]2 [+] Real (2*g) [*] y [=]Real (2*g*yG))
+      [&]((Real dy0[\<le>]Real 0 [&] x[\<le>]Real x1 [&] x[\<ge>]Real x0 [&] y[\<le>] Real y0 [&] y[\<ge>] Real y1)
+       [\<longrightarrow>](((x[-]Real cx)[**]2[+](y[-]Real cy)[**]2) [=] Real r [**]2 [&] x[\<ge>] Real cx[&] y[\<ge>] Real cy[&]v[**]2[\<ge>]Real vLo [&] v[**]2[\<le>]Real vHi [&] Real centLo[\<le>] Real cent[&]Real cent [\<le>]Real centHi [&] Real tanLo[\<le>]Real tan[&] Real tan[\<le>] Real tanHi))
+      [&](Real dy0[\<le>]Real 0)
+      [&](dx[=](y[-]Real cy)[div]Real r)
+      [&](dy[=](Real cx[-]x)[div]Real r)
+      [&](Real x1[>]Real x0)
+      [&](Real y1[<]Real y0)
+      [&](Real cy[\<le>]Real y1)
+      [&](Real cx[\<le>]Real x0)
+      [&](Real r[>]Real 0) "
 
 definition post3 :: fform where
-"post3 == (dx[=] (y[-]Con Real cy)[div]Con Real r)
-       [&](dy[=] (Con Real cx[-]x)[div]Con Real r)
-       [&](v[>]Con Real 0)
-       [&](v[**]2 [+] Con Real (2*g) [*] y [=]Con Real (2*g*yG))
-       [&](y[>]Con Real cy)
-       [&](((x[-]Con Real cx)[**]2[+](y[-]Con Real cy)[**]2) [=] Con Real r [**]2)"
+"post3 == (dx[=] (y[-]Real cy)[div]Real r)
+       [&](dy[=] (Real cx[-]x)[div]Real r)
+       [&](v[>]Real 0)
+       [&](v[**]2 [+] Real (2*g) [*] y [=]Real (2*g*yG))
+       [&](y[>]Real cy)
+       [&](((x[-]Real cx)[**]2[+](y[-]Real cy)[**]2) [=] Real r [**]2)"
 
 definition Inv3 :: fform where
 "Inv3 == Inv"
 
 
 lemma q1:"{pre3}
-         <[(''x'', R),(''y'',R),(''v'',R),(''dx'',R),(''dy'',R)]: [(v[*]dx),(v[*]dy),(dy[*]Con Real -g),((dy[*]v)[div]Con Real r),((Con Real 0[-]dx[*]v)[div]Con Real r)] && Inv & (x[\<le>]Con Real x1 [&] x[\<ge>]Con Real x0 [&] y[\<le>] Con Real y0 [&] y[\<ge>] Con Real y1)>
+         <[''x'', ''y'', ''v'', ''dx'', ''dy'']: [(v[*]dx),(v[*]dy),(dy[*]Real -g),((dy[*]v)[div]Real r),((Real 0[-]dx[*]v)[div]Real r)] && Inv & (x[\<le>]Real x1 [&] x[\<ge>]Real x0 [&] y[\<le>] Real y0 [&] y[\<ge>] Real y1)>
           {post3;(elE 0 [[|]] (almost post3))}"
   sorry
 
 definition pre4 :: fform where
-"pre4 == (Con Real g[\<ge>] Con Real 0)
-      [&](v[>]Con Real 0)
-      [&](v[**]2 [+] Con Real (2*g) [*] y [=]Con Real (2*g*yG))
-      [&]((Con Real dy0[\<ge>]Con Real 0 [&] x[\<le>]Con Real x1 [&] x[\<ge>]Con Real x0 [&] y[\<le>] Con Real y0 [&] y[\<ge>] Con Real y1)
-         [\<longrightarrow>](((x[-]Con Real cx)[**]2[+](y[-]Con Real cy)[**]2) [=] Con Real r [**]2 [&] x[\<ge>] Con Real cx[&] y[\<ge>] Con Real cy[&]v[**]2[\<ge>]Con Real vLo [&] v[**]2[\<le>]Con Real vHi [&] Con Real centLo[\<le>] Con Real cent[&]Con Real cent [\<le>]Con Real centHi [&] Con Real tanLo[\<le>]Con Real tan[&] Con Real tan[\<le>] Con Real tanHi))
-      [&](Con Real dy0[\<ge>]Con Real 0)
-      [&](dx[=](Con Real cy[-]y)[div]Con Real r)
-      [&](dy[=](x[-]Con Real cx)[div]Con Real r)
-      [&](Con Real x1[>]Con Real x0)
-      [&](Con Real y1[<]Con Real y0)
-      [&](Con Real r[>]Con Real 0)
-      [&](Con Real cy[\<le>]Con Real y1)
-      [&](Con Real cx[\<le>]Con Real x0)
-      [&]((x[\<le>]Con Real x1 [&] x[\<ge>]Con Real x0 [&] y[\<le>] Con Real y0 [&] y[\<ge>] Con Real y1)[\<longrightarrow>](v[**]2)[div]Con Real 2[>]Con Real g[*](Con Real y0[-]y))"
+"pre4 == (Real g[\<ge>] Real 0)
+      [&](v[>]Real 0)
+      [&](v[**]2 [+] Real (2*g) [*] y [=]Real (2*g*yG))
+      [&]((Real dy0[\<ge>]Real 0 [&] x[\<le>]Real x1 [&] x[\<ge>]Real x0 [&] y[\<le>] Real y0 [&] y[\<ge>] Real y1)
+         [\<longrightarrow>](((x[-]Real cx)[**]2[+](y[-]Real cy)[**]2) [=] Real r [**]2 [&] x[\<ge>] Real cx[&] y[\<ge>] Real cy[&]v[**]2[\<ge>]Real vLo [&] v[**]2[\<le>]Real vHi [&] Real centLo[\<le>] Real cent[&]Real cent [\<le>]Real centHi [&] Real tanLo[\<le>]Real tan[&] Real tan[\<le>] Real tanHi))
+      [&](Real dy0[\<ge>]Real 0)
+      [&](dx[=](Real cy[-]y)[div]Real r)
+      [&](dy[=](x[-]Real cx)[div]Real r)
+      [&](Real x1[>]Real x0)
+      [&](Real y1[<]Real y0)
+      [&](Real r[>]Real 0)
+      [&](Real cy[\<le>]Real y1)
+      [&](Real cx[\<le>]Real x0)
+      [&]((x[\<le>]Real x1 [&] x[\<ge>]Real x0 [&] y[\<le>] Real y0 [&] y[\<ge>] Real y1)[\<longrightarrow>](v[**]2)[div]Real 2[>]Real g[*](Real y0[-]y))"
       
 definition post4 :: fform where
-"post4 == (dx[=](Con Real cy[-]y)[div]Con Real r)
-       [&](dy[=](x[-]Con Real cx)[div]Con Real r)
-       [&](v[>]Con Real 0)
-       [&](v[**]2 [+] Con Real (2*g) [*] y [=]Con Real (2*g*yG))
-       [&](y[>]Con Real cy)
-       [&](((x[-]Con Real cx)[**]2[+](y[-]Con Real cy)[**]2) [=] Con Real r [**]2)"
+"post4 == (dx[=](Real cy[-]y)[div]Real r)
+       [&](dy[=](x[-]Real cx)[div]Real r)
+       [&](v[>]Real 0)
+       [&](v[**]2 [+] Real (2*g) [*] y [=]Real (2*g*yG))
+       [&](y[>]Real cy)
+       [&](((x[-]Real cx)[**]2[+](y[-]Real cy)[**]2) [=] Real r [**]2)"
 
 definition Inv4 :: fform where
 "Inv4 == Inv"
 
 
 lemma q1cw:"{pre4}
-         <[(''x'', R),(''y'',R),(''v'',R),(''dx'',R),(''dy'',R)]: [(v[*]dx),(v[*]dy),(dy[*]Con Real -g),((Con Real 0[-]dy[*]v)[div]Con Real r),((dx[*]v)[div]Con Real r)] && Inv & (x[\<le>]Con Real x1 [&] x[\<ge>]Con Real x0 [&] y[\<le>] Con Real y0 [&] y[\<ge>] Con Real y1)>
+         <[''x'', ''y'', ''v'', ''dx'', ''dy'']: [(v[*]dx),(v[*]dy),(dy[*]Real -g),((Real 0[-]dy[*]v)[div]Real r),((dx[*]v)[div]Real r)] && Inv & (x[\<le>]Real x1 [&] x[\<ge>]Real x0 [&] y[\<le>] Real y0 [&] y[\<ge>] Real y1)>
           {post4;(elE 0 [[|]] (almost post4))}"
   sorry
 
 
 definition pre5 :: fform where
-"pre5 == (Con Real g[\<ge>] Con Real 0)
-      [&](v[>]Con Real 0)
-      [&](v[**]2 [+] Con Real (2*g) [*] y [=]Con Real (2*g*yG))
-      [&]((Con Real dy0[\<ge>]Con Real 0 [&] x[\<le>]Con Real x1 [&] x[\<ge>]Con Real x0 [&] y[\<le>] Con Real y1 [&] y[\<ge>] Con Real y0)
-         [\<longrightarrow>](((x[-]Con Real cx)[**]2[+](y[-]Con Real cy)[**]2) [=] Con Real r [**]2 [&] x[\<le>] Con Real cx[&] y[\<ge>] Con Real cy[&]v[**]2[\<ge>]Con Real vLo [&] v[**]2[\<le>]Con Real vHi [&] Con Real centLo[\<le>] Con Real cent[&]Con Real cent [\<le>]Con Real centHi [&] Con Real tanLo[\<le>]Con Real tan[&] Con Real tan[\<le>] Con Real tanHi))
-      [&](Con Real dy0[\<ge>]Con Real 0)
-      [&](dx[=](y[-]Con Real cy)[div]Con Real r)
-      [&](dy[=](Con Real cx[-]x)[div]Con Real r)
-      [&](Con Real x1[>]Con Real x0)
-      [&](Con Real y1[>]Con Real y0)
-      [&](Con Real cy[\<le>]Con Real y0)
-      [&](Con Real x1[\<le>]Con Real cx)
-      [&](Con Real r[>]Con Real 0)
-      [&]((x[\<le>]Con Real x1 [&] x[\<ge>]Con Real x0 [&] y[\<le>] Con Real y1 [&] y[\<ge>] Con Real y0)[\<longrightarrow>](v[**]2)[div]Con Real 2[>]Con Real g[*](Con Real y1[-]y))"
+"pre5 == (Real g[\<ge>] Real 0)
+      [&](v[>]Real 0)
+      [&](v[**]2 [+] Real (2*g) [*] y [=]Real (2*g*yG))
+      [&]((Real dy0[\<ge>]Real 0 [&] x[\<le>]Real x1 [&] x[\<ge>]Real x0 [&] y[\<le>] Real y1 [&] y[\<ge>] Real y0)
+         [\<longrightarrow>](((x[-]Real cx)[**]2[+](y[-]Real cy)[**]2) [=] Real r [**]2 [&] x[\<le>] Real cx[&] y[\<ge>] Real cy[&]v[**]2[\<ge>]Real vLo [&] v[**]2[\<le>]Real vHi [&] Real centLo[\<le>] Real cent[&]Real cent [\<le>]Real centHi [&] Real tanLo[\<le>]Real tan[&] Real tan[\<le>] Real tanHi))
+      [&](Real dy0[\<ge>]Real 0)
+      [&](dx[=](y[-]Real cy)[div]Real r)
+      [&](dy[=](Real cx[-]x)[div]Real r)
+      [&](Real x1[>]Real x0)
+      [&](Real y1[>]Real y0)
+      [&](Real cy[\<le>]Real y0)
+      [&](Real x1[\<le>]Real cx)
+      [&](Real r[>]Real 0)
+      [&]((x[\<le>]Real x1 [&] x[\<ge>]Real x0 [&] y[\<le>] Real y1 [&] y[\<ge>] Real y0)[\<longrightarrow>](v[**]2)[div]Real 2[>]Real g[*](Real y1[-]y))"
 
 definition post5 :: fform where
-"post5 == (dx[=](y[-]Con Real cy)[div]Con Real r)
-       [&](dy[=](Con Real cx[-]x)[div]Con Real r)
-       [&](v[>]Con Real 0)
-       [&](v[**]2 [+] Con Real (2*g) [*] y [=]Con Real (2*g*yG))
-       [&](x[\<le>]Con Real cx)
-       [&](Con Real cy[\<le>]y)
-       [&](((x[-]Con Real cx)[**]2[+](y[-]Con Real cy)[**]2) [=] Con Real r [**]2)"
+"post5 == (dx[=](y[-]Real cy)[div]Real r)
+       [&](dy[=](Real cx[-]x)[div]Real r)
+       [&](v[>]Real 0)
+       [&](v[**]2 [+] Real (2*g) [*] y [=]Real (2*g*yG))
+       [&](x[\<le>]Real cx)
+       [&](Real cy[\<le>]y)
+       [&](((x[-]Real cx)[**]2[+](y[-]Real cy)[**]2) [=] Real r [**]2)"
 
 definition Inv5 :: fform where
 "Inv5 == Inv"
 
 
 lemma q2:"{pre5}
-         <[(''x'', R),(''y'',R),(''v'',R),(''dx'',R),(''dy'',R)]: [(v[*]dx),(v[*]dy),(dy[*]Con Real -g),((dy[*]v)[div]Con Real r),((Con Real 0[-]dx[*]v)[div]Con Real r)] && Inv & (x[\<le>]Con Real x1 [&] x[\<ge>]Con Real x0 [&] y[\<le>] Con Real y1 [&] y[\<ge>] Con Real y0)>
+         <[''x'', ''y'', ''v'', ''dx'', ''dy'']: [(v[*]dx),(v[*]dy),(dy[*]Real -g),((dy[*]v)[div]Real r),((Real 0[-]dx[*]v)[div]Real r)] && Inv & (x[\<le>]Real x1 [&] x[\<ge>]Real x0 [&] y[\<le>] Real y1 [&] y[\<ge>] Real y0)>
           {post5;(elE 0 [[|]] (almost post5))}"
   sorry
 
