lunarlander/goal.thy
@@ -4,45 +4,45 @@ begin
 
 (*The safety property to prove.*)
 definition safeProp :: fform where
-"safeProp == (plant_v1_1 [+](Con Real 2)) [<] (Con Real 0.05) [&] (plant_v1_1 [+] (Con Real 2)) [>] (Con Real -0.05)"
+"safeProp == (plant_v1_1 [+](Real 2)) [<] (Real 0.05) [&] (plant_v1_1 [+] (Real 2)) [>] (Real -0.05)"
 
 (*The system clock is always positive.*)
 axiomatization where
-Clock : "\<forall> s. (t [\<ge>] Con Real 0) s"
+Clock : "\<forall> s. (t [\<ge>] Real 0) s"
 
 
 (*The following lists the constraints for solving the differential invariants for the 
 differential equations.*)
 (*The invariant guarantees the postcondition.*)
 definition cons1 :: fform where 
-"cons1 \<equiv> ((t [\<ge>]Con Real 0 [&] t [\<le>] Con Real 0.128 [&] Inv) [\<longrightarrow>]  safeProp)"
+"cons1 \<equiv> ((t [\<ge>]Real 0 [&] t [\<le>] Real 0.128 [&] Inv) [\<longrightarrow>]  safeProp)"
 (*Initialization:the initial state guarantees the invariant;
 and Computation: the computation guarantees the invariant.*)
 definition cons2 :: fform where 
-"cons2 \<equiv> ((plant_v1_1[=](Con Real -2) [&] plant_m1_1[=](Con Real 1250) 
-    [&] control_1[=](Con Real (4055/2)) [&] t[=](Con Real 0)) [\<longrightarrow>] Inv)"
+"cons2 \<equiv> ((plant_v1_1[=](Real -2) [&] plant_m1_1[=](Real 1250) 
+    [&] control_1[=](Real (4055/2)) [&] t[=](Real 0)) [\<longrightarrow>] Inv)"
 (*The core parts: the discrete computation and differential equations garantee the invariants. *)
 definition cons31 :: fform where
-"cons31 == (((t [=](Con Real (16 / 125))) [&] Inv) [\<longrightarrow>] (Inv \<lbrakk>(Con Real 0), ''plant_t'', R\<rbrakk>))"
+"cons31 == (((t [=](Real (16 / 125))) [&] Inv) [\<longrightarrow>] (Inv \<lbrakk>(Real 0), ''plant_t''\<rbrakk>))"
 
 definition cons31_aux :: fform where
-"cons31_aux == \<lambda> s. ((t [=]Con Real (16 / 125) [&] Inv) s \<longrightarrow> Inv (\<lambda>(y, i). if y = ''plant_t'' \<and> i = R then evalE (Con Real 0) s else s (y, i)))" 
+"cons31_aux == \<lambda> s. ((t [=]Real (16 / 125) [&] Inv) s \<longrightarrow> Inv (\<lambda>y. if y = ''plant_t'' then evalE (Real 0) s else s y))" 
 
 
 definition cons32 :: fform where
 "cons32 == (Inv [\<longrightarrow>] (Inv \<lbrakk>(plant_m1_1 [*]
-                                   (Con Real (811 / 500) [-] Con Real (1 / 100) [*] (control_1 [div] plant_m1_1 [-] Con Real (811 / 500)) [-]
-                                    Con Real (3 / 5) [*] (plant_v1_1 [+] Con Real 2))), ''control_1'', R\<rbrakk>))"
+                                   (Real (811 / 500) [-] Real (1 / 100) [*] (control_1 [div] plant_m1_1 [-] Real (811 / 500)) [-]
+                                    Real (3 / 5) [*] (plant_v1_1 [+] Real 2))), ''control_1''\<rbrakk>))"
  
 
 definition cons32_aux :: fform where
 "cons32_aux == \<lambda> s. (Inv s \<longrightarrow>
-               Inv (\<lambda>(y, i). if (y = ''control_1'' \<and> i = R)
+               Inv (\<lambda>y. if y = ''control_1''
                        then (evalE (plant_m1_1 [*]
-                                   (Con Real (811 / 500) [-] Con Real (1 / 100) [*] (control_1 [div] plant_m1_1 [-] Con Real (811 / 500)) [-]
-                                    Con Real (3 / 5) [*] (plant_v1_1 [+] Con Real 2)))
+                                   (Real (811 / 500) [-] Real (1 / 100) [*] (control_1 [div] plant_m1_1 [-] Real (811 / 500)) [-]
+                                    Real (3 / 5) [*] (plant_v1_1 [+] Real 2)))
                              s)
-                       else s (y, i)))" 
+                       else s y))" 
 definition cons4 :: fform where 
 "cons4 \<equiv>  exeFlow(PC_Diff11) (Inv)  [\<longrightarrow>]  Inv"
 definition cons5 :: fform where 
@@ -72,13 +72,13 @@ done
 (**You can uncomment the above lines, if you have  Mathematica, Matlab, Yalmip and SDPT3 installed. "Sorry" will go away.**)
 sorry
 
-lemma constraint11: "\<forall> s. (t [\<ge>] Con Real 0 [&] t [\<le>] Con Real (16 / 125) [&] Inv) s \<longrightarrow> safeProp s"
+lemma constraint11: "\<forall> s. (t [\<ge>] Real 0 [&] t [\<le>] Real (16 / 125) [&] Inv) s \<longrightarrow> safeProp s"
 apply (cut_tac allCons)
 apply (simp add:cons1_def)
 by (metis fAnd_def fImp_def)
 
 
-lemma constraint1: "\<forall> s. (t [\<le>]Con Real (16 / 125) [&] Inv) s \<longrightarrow> safeProp s"
+lemma constraint1: "\<forall> s. (t [\<le>]Real (16 / 125) [&] Inv) s \<longrightarrow> safeProp s"
 apply (cut_tac allCons)
 apply (cut_tac Clock)
 by (metis constraint11 fAnd_def)
@@ -86,23 +86,23 @@ by (metis constraint11 fAnd_def)
 
 
 
-lemma constraint2: "\<forall> s. (plant_v1_1[=](Con Real -2) [&] plant_m1_1[=](Con Real 1250) 
-    [&] control_1[=](Con Real (4055/2)) [&] t[=](Con Real 0)) s \<longrightarrow> Inv s"
+lemma constraint2: "\<forall> s. (plant_v1_1[=](Real -2) [&] plant_m1_1[=](Real 1250) 
+    [&] control_1[=](Real (4055/2)) [&] t[=](Real 0)) s \<longrightarrow> Inv s"
 apply (cut_tac allCons)
 apply (simp add:cons2_def)
 by (metis fAnd_def fImp_def)
 
 
-lemma constraint31: "\<forall> s. ((t [=]Con Real (16 / 125) [&] Inv) s \<longrightarrow> Inv (\<lambda>(y, i). if y = ''plant_t'' \<and> i = R then evalE (Con Real 0) s else s (y, i)))"
+lemma constraint31: "\<forall> s. ((t [=]Real (16 / 125) [&] Inv) s \<longrightarrow> Inv (\<lambda>y. if y = ''plant_t'' then evalE (Real 0) s else s y))"
 apply (cut_tac allCons)
   apply (simp add:cons31_def) 
 proof -
-  { fix vv :: "char list \<times> typeid \<Rightarrow> val"
+  { fix vv :: "char list \<Rightarrow> real"
     have "cons31_aux vv"
       by (metis allCons cons31_fact fAnd_def)
-    then have "\<not> (RVar ''plant_t''[=]Con Real (16 / 125) [&] Inv) vv \<or> Inv (\<lambda>(cs, t). if cs = ''plant_t'' \<and> t = R then evalE (Con Real 0) vv else vv (cs, t))"
+    then have "\<not> (RVar ''plant_t''[=]Real (16 / 125) [&] Inv) vv \<or> Inv (\<lambda>cs. if cs = ''plant_t'' then evalE (Real 0) vv else vv cs)"
       by (simp add: cons31_aux_def) }
-  then show "\<forall>f. (RVar ''plant_t''[=]Con Real (16 / 125) [&] Inv) f \<longrightarrow> Inv (\<lambda>(cs, t). if cs = ''plant_t'' \<and> t = R then evalE (Con Real 0) f else f (cs, t))"
+  then show "\<forall>f. (RVar ''plant_t''[=]Real (16 / 125) [&] Inv) f \<longrightarrow> Inv (\<lambda>cs. if cs = ''plant_t'' then evalE (Real 0) f else f cs)"
     by meson
 qed
 
@@ -111,12 +111,12 @@ qed
 
 
 lemma constraint32: "\<forall> s. (Inv s \<longrightarrow>
-               Inv (\<lambda>(y, i). if (y = ''control_1'' \<and> i = R)
+               Inv (\<lambda>y. if y = ''control_1''
                        then (evalE (plant_m1_1 [*]
-                                   (Con Real (811 / 500) [-] Con Real (1 / 100) [*] (control_1 [div] plant_m1_1 [-] Con Real (811 / 500)) [-]
-                                    Con Real (3 / 5) [*] (plant_v1_1 [+] Con Real 2)))
+                                   (Real (811 / 500) [-] Real (1 / 100) [*] (control_1 [div] plant_m1_1 [-] Real (811 / 500)) [-]
+                                    Real (3 / 5) [*] (plant_v1_1 [+] Real 2)))
                              s)
-                       else s (y, i)))"
+                       else s y))"
   apply (cut_tac allCons)
   apply (simp add:fAnd_def, auto)  
   apply (simp add:cons32_def fImp_def fSubForm_def)
@@ -138,17 +138,15 @@ by (metis fAnd_def fImp_def)
 declare elE_def [simp del]
 
 
-lemma factLess: "(RVar x [\<le>] Con Real r) s \<Longrightarrow>
-  (RVar x [\<ge>] Con Real r) s \<Longrightarrow>  (RVar x [=] Con Real r) s"
-  apply (simp add:fLessEqual_def fGreaterEqual_def fLess_def fEqual_def fOr_def)
-  apply (case_tac "s (x, R)", auto)
-  done 
+lemma factLess: "(RVar x [\<le>] Real r) s \<Longrightarrow>
+  (RVar x [\<ge>] Real r) s \<Longrightarrow>  (RVar x [=] Real r) s"
+  by (simp add:fLessEqual_def fGreaterEqual_def fLess_def fEqual_def fOr_def)
 
 
 (*Goal for the whole process.*)
 lemma goal : "{fTrue} PP {safeProp; (elE 0 [[|]] (almost safeProp))}"
 (*mono*)
-apply (cut_tac px="fTrue" and qx="t [\<le>] Con Real (16 / 125) [&] Inv" and Hx="(elE 0 [[|]] (almost (t [\<le>] Con Real (16 / 125) [&] Inv)))" in ConsequenceRule, auto)
+apply (cut_tac px="fTrue" and qx="t [\<le>] Real (16 / 125) [&] Inv" and Hx="(elE 0 [[|]] (almost (t [\<le>] Real (16 / 125) [&] Inv)))" in ConsequenceRule, auto)
 prefer 2
 apply (cut_tac constraint1, auto)
 prefer 2
@@ -156,19 +154,19 @@ apply (cut_tac constraint1, auto)
 apply (simp add:dOr_def almost_def, auto)
 apply (simp add:PP_def PC_Init_def PD_Init_def)
 (*separate into intialization and repetitive control*)
-apply (cut_tac m = "((plant_v1_1[=](Con Real -2)) [&] (plant_m1_1[=](Con Real 1250)) [&] (control_1[=](Con Real 2027.5)) [&] (t[=](Con Real 0)))" 
-           and  H = "elE 0"  and  G="(elE 0 [[|]] (almost (t [\<le>] Con Real (16 / 125) [&] Inv)))"  in SequentialRule, auto)
+apply (cut_tac m = "((plant_v1_1[=](Real -2)) [&] (plant_m1_1[=](Real 1250)) [&] (control_1[=](Real 2027.5)) [&] (t[=](Real 0)))" 
+           and  H = "elE 0"  and  G="(elE 0 [[|]] (almost (t [\<le>] Real (16 / 125) [&] Inv)))"  in SequentialRule, auto)
 (*Init*)
-apply (cut_tac m = "((plant_v1_1[=]Con (Real -2)) [&] (plant_m1_1[=]Con (Real 1250)))" 
+apply (cut_tac m = "((plant_v1_1[=] (Real -2)) [&] (plant_m1_1[=] (Real 1250)))" 
      and  H = "elE 0"  and  G = "elE 0" in SequentialRule, auto)
-apply (cut_tac m = "plant_v1_1[=]Con Real - 2"  and  H = "elE 0" and  G = "elE 0" in SequentialRule, auto)
+apply (cut_tac m = "plant_v1_1[=]Real - 2"  and  H = "elE 0" and  G = "elE 0" in SequentialRule, auto)
 apply (rule AssignRRule, auto) apply (simp add:fEqual_def)
-apply (cut_tac m = "plant_v1_1[=]Con Real - 2 [&] plant_m1_1[=]Con Real 1250" 
+apply (cut_tac m = "plant_v1_1[=]Real - 2 [&] plant_m1_1[=]Real 1250" 
    and  H = "elE 0" and  G = "elE 0" in SequentialRule, auto)
 apply (rule AssignRRule, auto) apply (simp add:fAnd_def fEqual_def)
 apply (rule AssignRRule, auto) apply (simp add:fAnd_def fEqual_def)
 apply (simp add:elE_def chop_def)+
-apply (cut_tac m = "((plant_v1_1[=](Con Real -2)) [&] (plant_m1_1[=](Con Real 1250)) [&] (control_1[=](Con Real 2027.5)))" 
+apply (cut_tac m = "((plant_v1_1[=](Real -2)) [&] (plant_m1_1[=](Real 1250)) [&] (control_1[=](Real 2027.5)))" 
            and  H = "elE 0" and  G = "elE 0" in SequentialRule, auto)
 apply (rule AssignRRule, auto) apply (simp add:fAnd_def fEqual_def)
 apply (rule AssignRRule, auto) apply (simp add:fAnd_def fEqual_def)
@@ -176,7 +174,7 @@ apply (simp add:elE_def chop_def)+
 prefer 2
 apply (simp add:elE_def dOr_def chop_def)
 (*Rep Part*)
-apply (cut_tac px="Inv [&] t[=](Con Real 0) [&] t [\<le>] Con Real (16 / 125)" and qx="Inv [&] t[=](Con Real 0) [&] t [\<le>] Con Real (16 / 125)" and Hx="(elE 0 [[|]] (almost (t [\<le>] Con Real (16 / 125) [&] Inv)))" in ConsequenceRule,auto)
+apply (cut_tac px="Inv [&] t[=](Real 0) [&] t [\<le>] Real (16 / 125)" and qx="Inv [&] t[=](Real 0) [&] t [\<le>] Real (16 / 125)" and Hx="(elE 0 [[|]] (almost (t [\<le>] Real (16 / 125) [&] Inv)))" in ConsequenceRule,auto)
 prefer 2
 apply (cut_tac constraint2, auto) apply (simp add:fAnd_def fLessEqual_def fOr_def fLess_def fEqual_def)
 prefer 2
@@ -184,25 +182,25 @@ apply (simp add:fAnd_def fLessEqual_def fOr_def fLess_def)
 prefer 2
 apply (simp add:elE_def dOr_def)
 apply (simp add:Inv3_def)
-apply (cut_tac I = "Inv [&] RVar ''plant_t''[=]Con Real 0 [&]
-     RVar ''plant_t''[\<le>]Con Real (16 / 125)" and
-     P = "(PC_Difff; (RVar ''plant_t'') := (Con Real 0); PD_Rep)" and 
-  H = "elE 0 [[|]] almost (RVar ''plant_t''[\<le>]Con Real (16 / 125) [&] Inv)" in RepetitionRule_a, auto)
-apply (cut_tac P = "(RVar ''plant_t''[\<le>]Con Real (16 / 125) [&] Inv)"
+apply (cut_tac I = "Inv [&] RVar ''plant_t''[=]Real 0 [&]
+     RVar ''plant_t''[\<le>]Real (16 / 125)" and
+     P = "(PC_Difff; (RVar ''plant_t'') := (Real 0); PD_Rep)" and 
+  H = "elE 0 [[|]] almost (RVar ''plant_t''[\<le>]Real (16 / 125) [&] Inv)" in RepetitionRule_a, auto)
+apply (cut_tac P = "(RVar ''plant_t''[\<le>]Real (16 / 125) [&] Inv)"
       and h = h and n = n and nd = m in chopfor, auto)
 prefer 2
-apply (cut_tac px = "Inv [&] RVar ''plant_t''[=]Con Real 0 [&]
-     RVar ''plant_t''[\<le>]Con Real (16 /125)" and 
-     qx = "Inv [&] RVar ''plant_t''[=]Con Real 0 [&]
-           RVar ''plant_t''[\<le>]Con Real (16 / 125)" and 
-     Hx = "elE 0 [[|]] (elE 0 [[|]] almost (RVar ''plant_t''[\<le>]Con Real (16 / 125) [&] Inv))" in ConsequenceRule, auto)
+apply (cut_tac px = "Inv [&] RVar ''plant_t''[=]Real 0 [&]
+     RVar ''plant_t''[\<le>]Real (16 /125)" and 
+     qx = "Inv [&] RVar ''plant_t''[=]Real 0 [&]
+           RVar ''plant_t''[\<le>]Real (16 / 125)" and 
+     Hx = "elE 0 [[|]] (elE 0 [[|]] almost (RVar ''plant_t''[\<le>]Real (16 / 125) [&] Inv))" in ConsequenceRule, auto)
 apply (simp add: dOr_def)
-apply (cut_tac m = "t [=] Con Real (16 / 125) [&] Inv" and
-    H = "(elE 0 [[|]] (almost (t [\<le>] Con Real (16 / 125) [&] Inv)))" and  
+apply (cut_tac m = "t [=] Real (16 / 125) [&] Inv" and
+    H = "(elE 0 [[|]] (almost (t [\<le>] Real (16 / 125) [&] Inv)))" and  
   G= "elE 0" in  SequentialRule, auto)
 prefer 2
 apply (simp add: PD_Rep_def)
-apply (cut_tac m = "t [=] Con Real 0 [&] Inv" and 
+apply (cut_tac m = "t [=] Real 0 [&] Inv" and 
     H = "elE 0" and  G= "elE 0" in  SequentialRule, auto)
 apply (rule AssignRRule, auto)
 apply (cut_tac constraint31, auto)
@@ -223,7 +221,7 @@ apply (rule ContinuousRuleGT, auto)
 apply (simp add:fLess_def fAnd_def fEqual_def) 
 apply (simp add:fAnd_def)
 apply (simp add:fAnd_def, auto)
-apply (cut_tac e = "RVar ''plant_t''" and f = "Con Real (16 / 125)" in Lessc)
+apply (cut_tac e = "RVar ''plant_t''" and f = "Real (16 / 125)" in Lessc)
 apply (rule factLess, auto) 
 apply (cut_tac constraint4)
 apply (simp add:PC_Diff11_def Inv1_def)
@@ -235,7 +233,7 @@ apply (rule ContinuousRuleGT, auto)
 apply (simp add:fLess_def fAnd_def fEqual_def) 
 apply (simp add:fAnd_def)
 apply (simp add:fAnd_def, auto)
-apply (cut_tac e = "RVar ''plant_t''" and f = "Con Real (16 / 125)" in Lessc)
+apply (cut_tac e = "RVar ''plant_t''" and f = "Real (16 / 125)" in Lessc)
 apply (rule factLess, auto) 
 apply (cut_tac constraint5)
 apply (simp add:PC_Diff22_def Inv2_def)
